proof for address_as_bytes

proof/correctness/Correctness_Address.ec
@@ -15,6 +15,14 @@ require import WArray4.
 require import Params Address Repr2 Utils2.
 require import XMSS_IMPL.
 
+lemma in_nth ['a] (x : 'a list) (P : 'a -> bool) :
+    (forall (x0 : 'a ), x0 \in x => P x0) <=>
+    forall (k : int), 0 <= k < size x => P (nth witness x k).
+proof.
+split ; smt(@List). (* Without the split, smt doesnt work *)
+qed.
+
+
 lemma zero_addr_op_impl (address : adrs) :
     hoare[M(Syscall)._zero_address : true ==> res = zero_addr].
 proof.
@@ -41,89 +49,103 @@ lemma zero_addr_res (address : adrs) :
     phoare[M(Syscall)._zero_address : true ==> res = zero_addr] = 1%r
       by conseq zero_addr_ll (zero_addr_op_impl address) => //=. 
 
+op W32toBytes (x : W32.t) : W8.t list = rev (to_list (W4u8.unpack8 x)).
+
+op addrToBytes (a : adrs) : W8.t list = flatten (map W32toBytes (to_list a)).
+
+
 lemma u32_to_bytes_correct (x : W32.t) :
-    hoare [M(Syscall).__u32_to_bytes : arg.`2 = x ==> to_list res = W32toBytes x].
+    phoare [
+      M(Syscall).__u32_to_bytes : 
+      arg.`2 = x 
+      ==>  
+      to_list res = W32toBytes x
+    ] = 1%r.
 proof.
 proc.
 auto => /> &hr.
-rewrite /W32toBytes.
 apply (eq_from_nth witness).
-  + rewrite size_to_list size_map size_chunk //. 
-rewrite size_to_list => i?. 
-rewrite get_to_list initiE // (nth_map witness).
-  + rewrite size_chunk //. 
-rewrite /BSWAP_32 => />.
-rewrite ifT // /chunk nth_mkseq /(\bits8) => />.
+  + by rewrite size_to_list size_rev size_to_list.
+rewrite size_to_list // => i?.
+rewrite !get_to_list initiE //.
+rewrite /get8 /set32_direct initiE //= ifT 1:/# bits8E /=.
 rewrite wordP => j?.
-rewrite initiE // /(\o) /= /bits2w => />.
-rewrite initiE // nth_take // 1:/# nth_drop 1,2:/# /w2bits nth_mkseq 1:/# /= /unpack8 /=.
-rewrite pack4E initiE 1:/# //= /(\bits8).
-rewrite get_of_list 1:/# /= nth_rev.
+rewrite initiE //= /BSWAP_32 /(\o) pack4E initiE 1:/# /= get_of_list 1:/#.
+rewrite nth_rev.
   + rewrite size_to_list /#.
-rewrite size_to_list => />.
-rewrite initiE 1:/# /= initiE 1:/# /=.
-congr.
-(* Isto e verdade ?? *)
-admit.
+congr => [| /#].
+rewrite !get_to_list !size_to_list.
+rewrite nth_rev.
+  + rewrite size_to_list /#.
+rewrite size_to_list.
+rewrite /to_list nth_mkseq 1:/# /=.
+congr => /#.
 qed.
 
-lemma _addr_to_bytes_correctness (x : W32.t Array8.t) : 
+lemma addr_to_bytes_correctness (x : W32.t Array8.t) : 
     n = 32 =>
-    hoare[M(Syscall).__addr_to_bytes : 
-        arg.`2 = x ==> to_list res = val (addr_to_bytes x)].
+    phoare[
+        M(Syscall).__addr_to_bytes : 
+        arg.`2 = x 
+        ==> 
+        to_list res = flatten (map W32toBytes (to_list x))
+] = 1%r.
 proof.
 move => n_val.
 proc.
-while (
-  #pre /\
+while ( 
+  addr = x /\
   0 <= i <= 8 /\
-  forall (k : int), 0 <= k < 4*i => addr_as_bytes.[k] = nth witness (val (addr_to_bytes x)) k
-).
-    + seq 2 : (#pre /\ to_list buf = W32toBytes addr.[i]).
-         * ecall (u32_to_bytes_correct addr.[i]); auto => />. 
-      auto => /> &hr H0 H1 H2 H3 H4. 
-      do split; 1,2: by smt(). 
-      move => k??.
-      rewrite initiE 1:/# => />. 
-      case (4 * i{hr} <= k < 4 * i{hr} + 4) => *.
-         * rewrite -get_to_list H4 /W32toBytes /addr_to_bytes.
-           rewrite (nth_map witness); [rewrite size_chunk // size_w2bits /# |] => />.
-           rewrite insubdK.  
-              - rewrite /P /BitsToBytes size_map size_chunk // size_flatten sumzE BIA.big_map /(\o) //=. 
-                rewrite -(StdBigop.Bigint.BIA.eq_big_seq (fun _ => 32)) /=. 
-                      + admit.
-                rewrite big_constz count_predT size_mkseq n_val /#.
-           rewrite /BitsToBytes. 
-           rewrite (nth_map witness); [rewrite size_iota size_w2bits /# |].
-           rewrite size_w2bits nth_iota 1:/# => />.
-           rewrite wordP => j?.
-           rewrite (nth_map witness). 
-              - rewrite size_chunk // size_flatten sumzE BIA.big_map /(\o) //=. 
-                rewrite -(StdBigop.Bigint.BIA.eq_big_seq (fun _ => 32)).
-                      + admit.
-                rewrite big_constz count_predT size_mkseq /#.
-           rewrite /chunk nth_mkseq => />.
-              - admit.
-           rewrite /w2bits.
-           admit.
-         * rewrite H2 // /#.
-    + auto => /> &hr.
-      split => [/# |].
-      move => addBytes j ???.
-      have ->: j = 8 by smt(). 
-      move => H.
-      apply (eq_from_nth witness).
-         * rewrite size_to_list valP n_val //.
-      rewrite size_to_list => k?. 
-      rewrite get_to_list H //. 
-qed.
+  sub addr_as_bytes 0 (4 * i) = 
+  sub_list (flatten (map W32toBytes (to_list x))) 0 (4 * i)
+)
+(8 - i); last first.
+  + auto => /> *; split.
+      - apply (eq_from_nth witness); first by rewrite size_sub // size_sub_list /#.
+        rewrite size_sub // /#.
+      - move => addrBytes i; split => [/# |].
+        move => ???; have ->: i = 8 by smt(). 
+        move => /= H.
+        apply (eq_from_nth witness).
+            * rewrite size_to_list size_flatten.
+              rewrite sumzE BIA.big_map /(\o) //=.
+              rewrite -(StdBigop.Bigint.BIA.eq_big_seq (fun _ => 4)) /=; last first.
+                +  rewrite big_constz count_predT size_map size_to_list /#.
+                   rewrite in_nth.
+                   rewrite size_map size_to_list /= => j?.
+                   rewrite (nth_map witness); first by rewrite size_to_list /#.
+                   rewrite /W32toBytes size_rev; first by rewrite size_to_list /#.
+        rewrite size_to_list => j?.
+        rewrite get_to_list. 
+        have ->: addrBytes.[j] =nth witness (sub addrBytes 0 32) j by rewrite nth_sub /#.
+        by rewrite H nth_sub_list.
 
-lemma addr_to_bytes_ll : islossless M(Syscall).__addr_to_bytes by proc; inline; while (true) (8 - i); auto => /> /#.
-
-lemma addr_to_bytes_correctness (x : W32.t Array8.t) : 
-    phoare[M(Syscall).__addr_to_bytes : arg.`2 = x ==> 
-      to_list res = val (addr_to_bytes x)] = 1%r.
-proof.
-proc.
-admit.
+  + auto => />. 
+    exists * addr.[i]; elim * => P.
+    call (u32_to_bytes_correct P).
+    auto => /> &hr H0 H1 H2 H3 result Hr *; do split; 1,2,4: by smt().
+    apply (eq_from_nth witness); first by rewrite size_sub_list 1:/# size_sub 1,2:/#.
+    rewrite size_sub 1:/# => j?.
+    rewrite nth_sub_list 1:/# (nth_flatten witness 4).
+       + pose X := (fun (s : W8.t list) => size s = 4).
+         pose Y := (map W32toBytes (to_list x)).
+         rewrite -(all_nthP X Y witness) /X /Y size_map => k?. 
+         by rewrite (nth_map witness) // /W32toBytes size_rev size_to_list.
+    rewrite nth_sub 1:/# initiE 1:/# /=.   
+    rewrite (nth_map witness); first by rewrite size_to_list /#.
+    rewrite /W32toBytes nth_rev; first by rewrite size_to_list /#.
+    rewrite get_to_list size_to_list /to_list nth_mkseq 1:/# /=.
+    case (4 * i{hr} <= j < 4 * i{hr} + 4) => ?.
+       + rewrite (: result.[j - 4 * i{hr}] = nth witness (to_list result) (j - 4 * i{hr})) 1:/# Hr /W32toBytes.
+         rewrite nth_rev; first by rewrite size_to_list /#.
+         rewrite size_to_list /to_list nth_mkseq 1:/# /= /#.  
+       + have ->: addr_as_bytes{hr}.[j] = nth witness (sub addr_as_bytes{hr} 0 (4 * i{hr})) j by rewrite nth_sub /#.
+         rewrite H2 nth_sub_list 1:/# (nth_flatten witness 4).
+           * pose X := (fun (s : W8.t list) => size s = 4).
+             pose Y := (map W32toBytes (to_list x)).
+             rewrite -(all_nthP X Y witness) /X /Y size_map => k?. 
+             by rewrite (nth_map witness) // /W32toBytes size_rev size_to_list.
+         rewrite (nth_map witness); first by rewrite size_to_list /#.
+         rewrite /W32toBytes nth_rev; first by rewrite size_to_list /#.
+         by rewrite get_to_list size_to_list /to_list nth_mkseq 1:/# /=.
 qed.
